stlc_cap_pure.v
@@ -144,13 +144,13 @@ Definition progress_statement := forall t T,
    creating an instance of E *)
 
 Inductive capsafe: typ -> Prop :=
-| capsafe_B: capsafe typ_base
-| capsafe_C_X: forall S T, caprod S -> capsafe (typ_arrow_closed S T)
-| capsafe_X_S: forall S T, capsafe T -> capsafe (typ_arrow_closed S T)
+| capsafe_base: capsafe typ_base
+| capsafe_eff_any: forall S T, caprod S -> capsafe (typ_arrow_closed S T)
+| capsafe_any_safe: forall S T, capsafe T -> capsafe (typ_arrow_closed S T)
 
 with caprod: typ -> Prop :=
- | caprod_E: caprod typ_eff
- | caprod_S_C: forall S T, capsafe S -> caprod T -> caprod (typ_arrow_closed S T).
+ | caprod_eff: caprod typ_eff
+ | caprod_safe_eff: forall S T, capsafe S -> caprod T -> caprod (typ_arrow_closed S T).
 
 Inductive healthy: ctx -> Prop :=
   | healthy_empty: healthy empty
@@ -616,9 +616,9 @@ Lemma healthy_env_term_capsafe: forall E t T,
 Proof. intros. inductions H0.
   apply *healthy_env_capsafe.
   pick_fresh x. forwards~ : H1 x. destruct* (capsafe_decidable V).
-    apply capsafe_X_S. apply* (H2 x). rewrite* (healthy_env_closed H).
+    apply capsafe_any_safe. apply* (H2 x). rewrite* (healthy_env_closed H).
       apply* healthy_push.
-      apply capsafe_C_X. apply* not_capsafe_caprod.
+      apply capsafe_eff_any. apply* not_capsafe_caprod.
   forwards~ : IHtyping1 H. forwards~ : IHtyping2 H. inversions* H0.
   lets*: capsafe_not_caprod S.
 Qed.
